books/centaur/gl/eval-g-base-help.lisp
@@ -20,11 +20,13 @@
  generic-geval-alt-def
  ((generic-geval-ev eval-g-base-ev)
   (generic-geval-ev-lst eval-g-base-ev-lst)
-  (generic-geval eval-g-base))
+  (generic-geval eval-g-base)
+  (generic-geval-list eval-g-base-list))
  :hints ('(:in-theory (e/d* (eval-g-base-ev-of-fncall-args
                              eval-g-base-apply-agrees-with-eval-g-base-ev)
                             (eval-g-base-apply))
-           :expand ((eval-g-base x env))))
+           :expand ((eval-g-base x env)
+                    (eval-g-base-list x env))))
          ;; :do-not-induct
          ;;   t
          ;;   :expand ((eval-g-base x env))))
@@ -36,7 +38,8 @@
  mk-g-boolean-correct
  ((generic-geval-ev eval-g-base-ev)
   (generic-geval-ev-lst eval-g-base-ev-lst)
-  (generic-geval eval-g-base)))
+  (generic-geval eval-g-base)
+  (generic-geval-list eval-g-base-list)))
 
 
 
@@ -45,14 +48,16 @@
  gtests-obj-correct
  ((generic-geval-ev eval-g-base-ev)
   (generic-geval-ev-lst eval-g-base-ev-lst)
-  (generic-geval eval-g-base)))
+  (generic-geval eval-g-base)
+  (generic-geval-list eval-g-base-list)))
 
 (acl2::def-functional-instance
  gtests-nonnil-correct-for-eval-g-base
  gtests-nonnil-correct
  ((generic-geval-ev eval-g-base-ev)
   (generic-geval-ev-lst eval-g-base-ev-lst)
-  (generic-geval eval-g-base)))
+  (generic-geval eval-g-base)
+  (generic-geval-list eval-g-base-list)))
 
 (local
  (progn
@@ -64,7 +69,8 @@
     mk-g-ite-correct
     ((generic-geval-ev eval-g-base-ev)
      (generic-geval-ev-lst eval-g-base-ev-lst)
-     (generic-geval eval-g-base)))
+     (generic-geval eval-g-base)
+  (generic-geval-list eval-g-base-list)))
 
 
    (acl2::def-functional-instance
@@ -72,28 +78,32 @@
     gobj-ite-merge-correct
     ((generic-geval-ev eval-g-base-ev)
      (generic-geval-ev-lst eval-g-base-ev-lst)
-     (generic-geval eval-g-base)))))
+     (generic-geval eval-g-base)
+  (generic-geval-list eval-g-base-list)))))
 
 (acl2::def-functional-instance
  eval-g-base-g-apply
  generic-geval-g-apply
  ((generic-geval-ev eval-g-base-ev)
   (generic-geval-ev-lst eval-g-base-ev-lst)
-  (generic-geval eval-g-base)))
+  (generic-geval eval-g-base)
+  (generic-geval-list eval-g-base-list)))
 
 (acl2::def-functional-instance
  general-consp-car-correct-for-eval-g-base
  general-consp-car-correct
  ((generic-geval-ev eval-g-base-ev)
   (generic-geval-ev-lst eval-g-base-ev-lst)
-  (generic-geval eval-g-base)))
+  (generic-geval eval-g-base)
+  (generic-geval-list eval-g-base-list)))
 
 (acl2::def-functional-instance
  general-consp-cdr-correct-for-eval-g-base
  general-consp-cdr-correct
  ((generic-geval-ev eval-g-base-ev)
   (generic-geval-ev-lst eval-g-base-ev-lst)
-  (generic-geval eval-g-base)))
+  (generic-geval eval-g-base)
+  (generic-geval-list eval-g-base-list)))
 
 (in-theory (disable general-consp-car-correct-for-eval-g-base
                     general-consp-cdr-correct-for-eval-g-base))
@@ -103,14 +113,16 @@
  generic-geval-cons
  ((generic-geval-ev eval-g-base-ev)
   (generic-geval-ev-lst eval-g-base-ev-lst)
-  (generic-geval eval-g-base)))
+  (generic-geval eval-g-base)
+  (generic-geval-list eval-g-base-list)))
 
 (acl2::def-functional-instance
  eval-g-base-non-cons
  generic-geval-non-cons
  ((generic-geval-ev eval-g-base-ev)
   (generic-geval-ev-lst eval-g-base-ev-lst)
-  (generic-geval eval-g-base)))
+  (generic-geval eval-g-base)
+  (generic-geval-list eval-g-base-list)))
 
 (in-theory (disable eval-g-base-non-cons))
 
@@ -119,49 +131,63 @@
 ;;  generic-geval-gobj-fix
 ;;  ((apply-stub eval-g-base-apply)
 ;;   (generic-geval-apply eval-g-base-apply)
-;;   (generic-geval eval-g-base)))
+;;   (generic-geval eval-g-base)
 
 (acl2::def-functional-instance
  general-concrete-obj-when-consp-for-eval-g-base
  general-concrete-obj-when-consp
  ((generic-geval-ev eval-g-base-ev)
   (generic-geval-ev-lst eval-g-base-ev-lst)
-  (generic-geval eval-g-base)))
+  (generic-geval eval-g-base)
+  (generic-geval-list eval-g-base-list)))
 
 (acl2::def-functional-instance
  not-general-numberp-not-acl2-numberp-for-eval-g-base
  not-general-numberp-not-acl2-numberp
  ((generic-geval-ev eval-g-base-ev)
   (generic-geval-ev-lst eval-g-base-ev-lst)
-  (generic-geval eval-g-base)))
+  (generic-geval eval-g-base)
+  (generic-geval-list eval-g-base-list)))
 
 (acl2::def-functional-instance
  mk-g-number-correct-for-eval-g-base
  mk-g-number-correct
  ((generic-geval-ev eval-g-base-ev)
   (generic-geval-ev-lst eval-g-base-ev-lst)
-  (generic-geval eval-g-base)))
+  (generic-geval eval-g-base)
+  (generic-geval-list eval-g-base-list)))
 
 (acl2::def-functional-instance
  mk-g-concrete-correct-for-eval-g-base
  mk-g-concrete-correct
  ((generic-geval-ev eval-g-base-ev)
   (generic-geval-ev-lst eval-g-base-ev-lst)
-  (generic-geval eval-g-base)))
+  (generic-geval eval-g-base)
+  (generic-geval-list eval-g-base-list)))
 
 (acl2::def-functional-instance
  g-concrete-quote-correct-for-eval-g-base
  g-concrete-quote-correct
  ((generic-geval-ev eval-g-base-ev)
   (generic-geval-ev-lst eval-g-base-ev-lst)
-  (generic-geval eval-g-base)))
+  (generic-geval eval-g-base)
+  (generic-geval-list eval-g-base-list)))
 
 (acl2::def-functional-instance
  eval-g-base-of-gl-cons
  generic-geval-gl-cons
  ((generic-geval-ev eval-g-base-ev)
   (generic-geval-ev-lst eval-g-base-ev-lst)
-  (generic-geval eval-g-base)))
+  (generic-geval eval-g-base)
+  (generic-geval-list eval-g-base-list)))
+
+(acl2::def-functional-instance
+ eval-g-base-list-of-gl-cons
+ generic-geval-list-gl-cons
+ ((generic-geval-ev eval-g-base-ev)
+  (generic-geval-ev-lst eval-g-base-ev-lst)
+  (generic-geval eval-g-base)
+  (generic-geval-list eval-g-base-list)))
 
 
 
